LeanALaCarte.lean
@@ -2,6 +2,5 @@ import LeanALaCarte.Basic
 import LeanALaCarte.CheckTranslation
 import LeanALaCarte.ExtendInd
 import LeanALaCarte.NewMap
-import LeanALaCarte.Tests
+import LeanALaCarte.Test
 import LeanALaCarte.NewMap
-import LeanALaCarte.ModDefTests
