LeanALaCarte/Test.lean
@@ -1,0 +1,2 @@
+import LeanALaCarte.Test.InductiveExtend
+import LeanALaCarte.Test.ModDef
